counting oracle api

src/computational_monads/simulation_semantics/constructions/counting_oracle.lean
@@ -14,22 +14,55 @@ The internal state of the oracle is exactly a `n : ℕ` giving the amount of que
 This value is always finite as the `oracle_comp` monad doesn't have unbounded recursion.
 -/
 
-open oracle_comp oracle_spec
+open oracle_comp oracle_spec sim_oracle
 
 variables {α β γ : Type} {spec spec' : oracle_spec}
 
 /-- Simulation oracle for counting the queries made during the computation,
 tracked via a `query_count`, whithout modifying the query calls themselves. -/
-def counting_oracle (spec : oracle_spec) : sim_oracle spec spec (query_count spec) :=
+@[inline, reducible] def counting_oracle (spec : oracle_spec) :
+  sim_oracle spec spec (query_count spec) :=
 ⟪query | λ qc i u t, qc.increment i 1, ∅⟫
 
 notation `countingₛₒ` := counting_oracle _
+
+lemma counting_oracle.def : (counting_oracle spec) =
+  ⟪query | λ qc i u t, qc.increment i 1, ∅⟫ := rfl
 
 instance counting_oracle.is_tracking : (counting_oracle spec).is_tracking :=
 tracking_oracle.is_tracking query _ ∅
 
 namespace counting_oracle
 
--- TODO
+lemma apply_eq {i : spec.ι} (t : spec.domain i) (qc : spec.query_count) :
+  countingₛₒ i (t, qc) = (λ u, (u, qc.increment i 1)) <$> (query i t) := rfl
+
+lemma answer_query_eq : (counting_oracle spec).answer_query = query := rfl
+
+lemma update_state_eq : (counting_oracle spec).update_state = λ qc i u t, qc.increment i 1 := rfl
+
+section simulate'
+
+variables (oa : oracle_comp spec α) (s : spec.query_count)
+
+@[pairwise_dist_equiv] lemma simulate'_dist_equiv : simulate' countingₛₒ oa s ≃ₚ oa :=
+is_tracking.simulate'_dist_equiv_self countingₛₒ oa s (λ i t, dist_equiv.rfl)
+
+@[simp] lemma support_simulate' : (simulate' countingₛₒ oa s).support = oa.support :=
+by pairwise_dist_equiv
+
+@[simp] lemma fin_support_simulate' : (simulate' countingₛₒ oa s).fin_support = oa.fin_support :=
+by pairwise_dist_equiv
+
+@[simp] lemma eval_dist_simulate' : ⁅simulate' countingₛₒ oa s⁆ = ⁅oa⁆ :=
+by pairwise_dist_equiv
+
+@[simp] lemma prob_output_simulate' (x : α) : ⁅= x | simulate' countingₛₒ oa s⁆ = ⁅= x | oa⁆ :=
+by pairwise_dist_equiv
+
+@[simp] lemma prob_event_simulate' (e : set α) : ⁅e | simulate' countingₛₒ oa s⁆ = ⁅e | oa⁆ :=
+by pairwise_dist_equiv
+
+end simulate'
 
 end counting_oracle
